spot/GC.SPOT.HeapExpansion.fst
@@ -724,6 +724,21 @@ let spot_promote_object_head_split_preserves_chunked_alloc_shape_single_chunk
   CheneyPreservation.promote_object_head_split_preserves_chunked_alloc_shape_single_chunk
     minor major obj fp wosize
 
+let spot_cheney_forward_one_split_ready_from_minor_demand_single_chunk
+  (minor: minor_state) (cs: cheney_state) (addr: U64.t)
+  : Lemma
+      (requires minor_wf minor /\
+                cs.cs_fp <> 0UL /\
+                SpecMajorAlloc.major_fl_head_wosize
+                  (MH.single_chunk_major_heap cs.cs_major) cs.cs_fp >=
+                PromotionDemand.minor_promotion_demand minor + 1)
+      (ensures
+        CheneyPreservation.cheney_forward_one_split_ready_single_chunk
+          minor cs addr)
+  =
+  CheneyPreservation.cheney_forward_one_split_ready_from_minor_demand_single_chunk
+    minor cs addr
+
 let spot_cheney_forward_one_head_split_preserves_chunked_alloc_shape_single_chunk
   (minor: minor_state) (cs: cheney_state) (addr: U64.t)
   : Lemma
@@ -859,6 +874,43 @@ let spot_cheney_promote_head_split_preserves_chunked_alloc_shape_single_chunk
            SpecAlloc.alloc_search_fuel = true))
   =
   CheneyPreservation.cheney_promote_head_split_preserves_chunked_alloc_shape_single_chunk
+    minor major fp roots
+
+let spot_cheney_promote_budgeted_head_split_preserves_chunked_alloc_shape_single_chunk
+  (minor: minor_state) (major: heap) (fp: U64.t) (roots: Seq.seq U64.t)
+  : Lemma
+      (requires minor_wf minor /\
+                SpecAlloc.alloc_search_fuel > 1 /\
+                fp <> 0UL /\
+                GenInv.chunked_major_alloc_shape
+                  (MH.single_chunk_major_heap major) fp
+                  SpecAlloc.alloc_search_fuel /\
+                SpecMajorAlloc.major_fl_chain_terminates
+                  (MH.single_chunk_major_heap major) fp
+                  SpecAlloc.alloc_search_fuel = true /\
+                SpecMajorAlloc.major_fl_head_wosize
+                  (MH.single_chunk_major_heap major) fp >=
+                  PromotionDemand.minor_promotion_demand minor + 1 /\
+                CheneyPreservation.cheney_promote_split_ready_single_chunk
+                  minor major fp roots)
+      (ensures
+        (let res = cheney_promote minor major fp roots in
+         let requests =
+           CheneyPreservation.cheney_forwarded_minor_requests
+             minor major fp roots in
+         let alloc_trace =
+           SpecMajorAllocMultiAlloc.dense_alloc_list_default_spec
+             major fp requests in
+         GenInv.chunked_major_alloc_shape
+           (MH.single_chunk_major_heap res.major_final) res.fp_final
+           SpecAlloc.alloc_search_fuel /\
+         SpecMajorAlloc.major_fl_chain_terminates
+           (MH.single_chunk_major_heap res.major_final) res.fp_final
+           SpecAlloc.alloc_search_fuel = true /\
+         SpecMajorAllocMultiAlloc.allocated_objects_nonzero
+           alloc_trace.dense_list_objs_out))
+  =
+  CheneyPreservation.cheney_promote_budgeted_head_split_preserves_chunked_alloc_shape_single_chunk
     minor major fp roots
 
 let spot_chunked_is_blue_preserved_by_expansion
